amend!

Docs/ContextualEmbedding/Extrinsic/CE.lean
@@ -19,26 +19,26 @@ deriving Repr, DecidableEq
 
 infixl:90 " :/: " => Ctx.Snoc
 
-inductive Index : Type where
-  | Top : Index
-  | Pop : Index -> Index
+inductive Index : Ctx -> Type where
+  | Top {ts : Ctx} {t : Ty} : Index (ts :/: t)
+  | Pop {ts : Ctx} {t' : Ty} : Index ts -> Index (ts :/: t')
 deriving Repr, DecidableEq
 open Index
 
-inductive STLC : Type where
-  | Var : Index -> STLC
-  | Star : STLC
-  | Lambda : Ty -> STLC -> STLC
-  | Apply : STLC -> STLC -> STLC
+inductive STLC : Ctx -> Type where
+  | Var (i : Index ts) : STLC ts
+  | Star : STLC ts
+  | Lambda (a : Ty) (body : STLC (ts :/: a)) : STLC ts
+  | Apply (fn : STLC ts) (arg : STLC ts) : STLC ts
 deriving Repr, DecidableEq
 open STLC
 
-inductive Lookup : Ctx -> Index -> Ty -> Type where
+inductive Lookup : (ts : Ctx) -> Index ts -> Ty -> Type where
   | Top {ts : Ctx} {t : Ty} : Lookup (ts :/: t) Top t
-  | Pop {ts : Ctx} {t t' : Ty} {i : Index} : Lookup ts i t -> Lookup (ts :/: t') (Pop i) t
+  | Pop {ts : Ctx} {t t' : Ty} {i : Index ts} : Lookup ts i t -> Lookup (ts :/: t') (Pop i) t
 deriving Repr
 
-inductive HasType : Ctx -> STLC -> Ty -> Type where
+inductive HasType : (ts : Ctx) -> STLC ts -> Ty -> Type where
   | Var : Lookup ts i t -> HasType ts (Var i) t
   | Star : HasType ts Star Unit
   | Lambda : HasType (ts :/: t1) e t2 -> HasType ts (Lambda t1 e) (t1 :-> t2)
@@ -51,7 +51,7 @@ deriving Repr, DecidableEq
 open ProxyTop
 
 class ReifyIndex (ts : Ctx) (ts' : Ctx) where
-  reify : ProxyTop ts -> Index
+  reify : ProxyTop ts -> Index ts'
 open ReifyIndex
 
 instance instReifyIndexRefl : ReifyIndex (ts :/: t) (ts :/: t) where
@@ -59,22 +59,22 @@ instance instReifyIndexRefl : ReifyIndex (ts :/: t) (ts :/: t) where
     | PTop => Top
 
 instance instReifyIndexSnoc [instRec : ReifyIndex ts1 ts2] : ReifyIndex ts1 (ts2 :/: t') where
-  reify := fun i => Pop (ReifyIndex.reify ts2 (self := instRec) i)
+  reify := fun i => Pop (ReifyIndex.reify (self := instRec) i)
 
-inductive STLCCtx : Type where
-  | CVar {ts ts' : Ctx} [inst : ReifyIndex ts ts'] : ProxyTop ts -> STLCCtx
-  | CStar : STLCCtx
-  | CLam {ts : Ctx} (a : Ty) : (ProxyTop (ts :/: a) -> STLCCtx) -> STLCCtx
-  | CApp : STLCCtx -> STLCCtx -> STLCCtx
+inductive STLCCtx : Ctx -> Type where
+  | CVar {ts ts' : Ctx} [inst : ReifyIndex ts ts'] (proxy : ProxyTop ts) : STLCCtx ts'
+  | CStar : STLCCtx ts
+  | CLam {ts : Ctx} (a : Ty) (body : ProxyTop (ts :/: a) -> STLCCtx (ts :/: a)) : STLCCtx ts
+  | CApp (fn : STLCCtx ts) (arg : STLCCtx ts) : STLCCtx ts
 open STLCCtx
 
 
 -- Unembed
 -----------
 
-def unembed : STLCCtx -> STLC
+def unembed : STLCCtx ts -> STLC ts
   | STLCCtx.CStar => STLC.Star
-  | @STLCCtx.CVar _ ts' inst proxy => STLC.Var (ReifyIndex.reify ts' (self := inst) proxy)
+  | @STLCCtx.CVar _ _ inst proxy => STLC.Var (ReifyIndex.reify (self := inst) proxy)
   | @STLCCtx.CLam ts a body => STLC.Lambda a (unembed (body (@PTop ts a)))
   | STLCCtx.CApp e1 e2 => STLC.Apply (unembed e1) (unembed e2)
 
@@ -94,113 +94,108 @@ def weakenPVar : ProxyVar ts' -> ProxyVar (ts' :/: t')
 def varTop : ProxyVar (ts :/: t) :=
   PVar (inst := instReifyIndexRefl) (@PTop ts t)
 
-def fromVar : ProxyVar ts' -> STLCCtx
+def fromVar : ProxyVar ts' -> STLCCtx ts'
   | @PVar _ _ inst proxy => STLCCtx.CVar (inst := inst) proxy
 
-def fromIndex : Lookup ts i t -> ProxyVar ts
-  | Lookup.Top => varTop
-  | Lookup.Pop i => weakenPVar (fromIndex i)
+def fromIndex : Index ts -> ProxyVar ts
+  | Top => varTop
+  | Pop i => weakenPVar (fromIndex i)
 
-def toCVar : Lookup ts i t -> STLCCtx :=
+def toCVar : Index ts -> STLCCtx ts :=
   fun i => fromVar (fromIndex i)
 
-inductive CtxHasType : Ctx -> STLCCtx -> Ty -> Type where
-  | CVar : (lookup : Lookup ts i t) -> CtxHasType ts (toCVar lookup) t
+inductive CtxHasType : (ts : Ctx) -> STLCCtx ts -> Ty -> Type where
+  | CVar : (lookup : Lookup ts i t) -> CtxHasType ts (toCVar i) t
   | CStar : CtxHasType ts CStar Unit
   | CLam : ((proxy : ProxyTop (ts :/: a)) -> CtxHasType (ts :/: a) (body proxy) b) ->
       CtxHasType ts (CLam (ts := ts) a body) (a :-> b)
   | CApp : CtxHasType ts e1 (a :-> b) -> CtxHasType ts e2 a -> CtxHasType ts (CApp e1 e2) b
 
-def contextualise : HasType ts e t -> STLCCtx
-  | HasType.Var i => toCVar i
-  | @HasType.Lambda ts a _ _ e => STLCCtx.CLam (ts := ts) a (fun _ => contextualise e)
-  | HasType.Apply e1 e2 => STLCCtx.CApp (contextualise e1) (contextualise e2)
-  | HasType.Star => STLCCtx.CStar
+def contextualise : STLC ts -> STLCCtx ts
+  | STLC.Var i => toCVar i
+  | STLC.Lambda a e => STLCCtx.CLam (ts := ts) a (fun _ => contextualise e)
+  | STLC.Apply e1 e2 => STLCCtx.CApp (contextualise e1) (contextualise e2)
+  | STLC.Star => STLCCtx.CStar
 
 --------------------------------------------
 --           Isomorphism proofs           --
 --------------------------------------------
 
-theorem indexIsoL (i : Lookup ts idx t)
-  : ReifyIndex.reify ts (self := (fromIndex i).2) (fromIndex i).3 = idx := by
+theorem indexIsoL (i : Index ts)
+  : ReifyIndex.reify (self := (fromIndex i).2) (fromIndex i).3 = i := by
   induction i with
   | Top => rfl
   | Pop i' ih =>
-      change Pop (ReifyIndex.reify _ (self := (fromIndex i').2) (fromIndex i').3) = Pop _
+      change Pop (ReifyIndex.reify (self := (fromIndex i').2) (fromIndex i').3) = Pop i'
       exact congrArg Pop ih
 
-theorem unembedToCVar (lookup : Lookup ts i t) : unembed (toCVar lookup) = STLC.Var i := by
-  induction lookup with
+theorem unembedToCVar (i : Index ts) : unembed (toCVar i) = STLC.Var i := by
+  induction i with
   | Top => rfl
-  | Pop lookup ih =>
-      change STLC.Var (Index.Pop (ReifyIndex.reify _ (self := (fromIndex lookup).2) (fromIndex lookup).3)) =
-        STLC.Var (Index.Pop _)
-      exact congrArg (fun index => STLC.Var (Index.Pop index)) (indexIsoL lookup)
+  | Pop i' ih =>
+      change STLC.Var (Index.Pop (ReifyIndex.reify (self := (fromIndex i').2) (fromIndex i').3)) =
+        STLC.Var (Index.Pop i')
+      exact congrArg (fun index => STLC.Var (Index.Pop index)) (indexIsoL i')
 
-theorem indexIsoR (lookup : Lookup ts i t)
-  : contextualise (HasType.Var lookup) = toCVar lookup := by
+theorem indexIsoR (i : Index ts)
+  : contextualise (STLC.Var i) = toCVar i := by
   rfl
 
 def unembedTyped : CtxHasType ts e t -> HasType ts (unembed e) t
-  | CtxHasType.CVar lookup => (unembedToCVar lookup).symm ▸ HasType.Var lookup
+  | CtxHasType.CVar lookup => by
+      rw [unembedToCVar]
+      exact HasType.Var lookup
   | CtxHasType.CStar => HasType.Star
   | @CtxHasType.CLam ts a _ _ bodyTyped =>
       HasType.Lambda (unembedTyped (bodyTyped (@PTop ts a)))
   | CtxHasType.CApp e1 e2 => HasType.Apply (unembedTyped e1) (unembedTyped e2)
 
-theorem isoL {h : HasType ts e t}
-  : unembed (contextualise h) = e := by
-  induction h with
+theorem isoL {e : STLC ts}
+  : unembed (contextualise e) = e := by
+  induction e with
   | Star => rfl
   | Apply e1 e2 ih1 ih2 => simp [contextualise, unembed, ih1, ih2]
-  | Lambda e ih => simp [contextualise, unembed, ih]
+  | Lambda a body ih => simp [contextualise, unembed, ih]
   | Var i =>
       simp [contextualise, toCVar, fromVar, unembed]
       exact indexIsoL i
 
-theorem isoL' {h : HasType ts e t}
-  : unembed (contextualise h) = e := by
-  induction h
+theorem isoL' {e : STLC ts}
+  : unembed (contextualise e) = e := by
+  induction e
     <;> simp [contextualise, unembed, *]
   case Var i =>
     simp [toCVar, fromVar, unembed]
     exact indexIsoL i
 
-theorem isoR {ts : Ctx} {e : STLCCtx} {t : Ty}
-  : (h : CtxHasType ts e t) -> contextualise (unembedTyped h) = e
-  | CtxHasType.CVar lookup => by
-      change contextualise ((unembedToCVar lookup).symm ▸ HasType.Var lookup) = toCVar lookup
-      calc
-        contextualise ((unembedToCVar lookup).symm ▸ HasType.Var lookup)
-            = contextualise (HasType.Var lookup) := by
-              have castContextualise {e1 e2 : STLC} (h : e1 = e2) (typed : HasType ts e1 t) :
-                  contextualise (h ▸ typed) = contextualise typed := by
-                cases h
-                rfl
-              exact castContextualise (unembedToCVar lookup).symm (HasType.Var lookup)
-        _ = toCVar lookup := indexIsoR lookup
-  | CtxHasType.CStar => rfl
-  | @CtxHasType.CLam ts a _ _ bodyTyped => by
-      simp [unembedTyped, contextualise, unembed]
+theorem isoR {h : CtxHasType ts e t}
+  : contextualise (unembed e) = e := by
+  induction h with
+  | CVar lookup =>
+      rw [unembedToCVar]
+      rfl
+  | CStar => rfl
+  | CLam bodyTyped ih =>
+      simp [unembed, contextualise]
       funext x
       cases x
-      simp [isoR (bodyTyped (@PTop ts a))]
-  | CtxHasType.CApp e1 e2 => by
-      simp [unembedTyped, contextualise, isoR e1, isoR e2]
+      simp [ih]
+  | CApp e1 e2 ih1 ih2 =>
+      simp [unembed, contextualise, ih1, ih2]
 
 theorem isoR' {h : CtxHasType ts e t}
-  : contextualise (unembedTyped h) = e := isoR h
+  : contextualise (unembed e) = e := isoR (h := h)
 
 -- Examples
 ------------
 
-def showSTLCCtx : STLCCtx -> String
-  | @STLCCtx.CVar _ ts' inst proxy => "CVar " ++ reprStr proxy ++ "[reified = " ++ reprStr (ReifyIndex.reify ts' (self := inst) proxy) ++ "]"
+def showSTLCCtx : STLCCtx ts -> String
+  | @STLCCtx.CVar _ _ inst proxy => "CVar " ++ reprStr proxy ++ "[reified = " ++ reprStr (ReifyIndex.reify (self := inst) proxy) ++ "]"
   | STLCCtx.CStar => "CStar"
   | @STLCCtx.CLam ts a body => "CLam (\\<ProxyTop> -> " ++ showSTLCCtx (body (@PTop ts a)) ++ ")"
   | STLCCtx.CApp f x => "CApp (" ++ showSTLCCtx f ++ ") (" ++ showSTLCCtx x ++ ")"
 
-def idSTLC {ts : Ctx} {a : Ty} : STLCCtx :=
+def idSTLC {ts : Ctx} {a : Ty} : STLCCtx ts :=
   STLCCtx.CLam (ts := ts) a (fun x => STLCCtx.CVar (ts' := ts :/: a) x)
 
 def idSTLCTyped {ts : Ctx} {a : Ty} : CtxHasType ts (@idSTLC ts a) (a :-> a) :=
@@ -214,10 +209,10 @@ def idSTLCTyped' := @idSTLCTyped Ctx.Empty Unit
 #check idSTLC
 #eval showSTLCCtx idSTLC'
 #eval unembed idSTLC'
-#eval showSTLCCtx (contextualise (unembedTyped idSTLCTyped'))
-#eval unembed (contextualise (unembedTyped idSTLCTyped'))
+#eval showSTLCCtx (contextualise (unembed idSTLC'))
+#eval unembed (contextualise (unembed idSTLC'))
 
-def const {ts : Ctx} {a b : Ty} : STLCCtx :=
+def const {ts : Ctx} {a b : Ty} : STLCCtx ts :=
   STLCCtx.CLam (ts := ts) a
     (fun x => STLCCtx.CLam (ts := ts :/: a) b
       (fun _y => STLCCtx.CVar (ts' := (ts :/: a) :/: b) x))
@@ -233,10 +228,10 @@ def constTyped' := @constTyped Ctx.Empty Unit Unit
 
 #eval showSTLCCtx const'
 #eval unembed const'
-#eval showSTLCCtx (contextualise (unembedTyped constTyped'))
-#eval unembed (contextualise (unembedTyped constTyped'))
+#eval showSTLCCtx (contextualise (unembed const'))
+#eval unembed (contextualise (unembed const'))
 
-def flipConst {ts : Ctx} {a b : Ty} : STLCCtx :=
+def flipConst {ts : Ctx} {a b : Ty} : STLCCtx ts :=
   STLCCtx.CLam (ts := ts) a
     (fun _x => STLCCtx.CLam (ts := ts :/: a) b
       (fun y => STLCCtx.CVar (ts' := (ts :/: a) :/: b) y))
@@ -253,10 +248,10 @@ def flipConstTyped' := @flipConstTyped Ctx.Empty Unit Unit
 #check flipConst
 #eval showSTLCCtx flipConst'
 #eval unembed flipConst'
-#eval showSTLCCtx (contextualise (unembedTyped flipConstTyped'))
-#eval unembed (contextualise (unembedTyped flipConstTyped'))
+#eval showSTLCCtx (contextualise (unembed flipConst'))
+#eval unembed (contextualise (unembed flipConst'))
 
-def const5 {ts : Ctx} {a b c d e : Ty} : STLCCtx :=
+def const5 {ts : Ctx} {a b c d e : Ty} : STLCCtx ts :=
   STLCCtx.CLam (ts := ts) a (fun x1 =>
     STLCCtx.CLam (ts := ts :/: a) b (fun _x2 =>
       STLCCtx.CLam (ts := (ts :/: a) :/: b) c (fun _x3 =>
@@ -280,8 +275,8 @@ def const5Typed' := @const5Typed Ctx.Empty Unit Unit Unit Unit Unit
 
 #eval showSTLCCtx const5'
 #eval unembed const5'
-#eval showSTLCCtx (contextualise (unembedTyped const5Typed'))
-#eval unembed (contextualise (unembedTyped const5Typed'))
+#eval showSTLCCtx (contextualise (unembed const5'))
+#eval unembed (contextualise (unembed const5'))
 
 
 -- Examples in theorems
@@ -293,9 +288,7 @@ example {ts : Ctx} {a : Ty}
   rfl
 
 example {ts : Ctx} {a : Ty}
-  : @contextualise ts (STLC.Lambda a (STLC.Var Index.Top)) (a :-> a)
-    (@HasType.Lambda ts a (STLC.Var Index.Top) a
-      (@HasType.Var (ts :/: a) Index.Top a (@Lookup.Top ts a))) =
+  : @contextualise ts (STLC.Lambda a (STLC.Var Index.Top)) =
     @STLCCtx.CLam ts a (fun y => STLCCtx.CVar (ts' := ts :/: a) y) := by
   simp [contextualise, toCVar, fromIndex, fromVar]
   funext x
